Cslib/Languages/LambdaCalculus/Named/Untyped/Properties.lean
@@ -1,7 +1,7 @@
 /-
 Copyright (c) 2026 Haoxuan Yin. All rights reserved.
 Released under Apache 2.0 license as described in the file LICENSE.
-Authors: Haoxuan Yin
+Authors: Haoxuan Yin, Fabrizio Montesi
 -/
 
 module
@@ -21,25 +21,25 @@ namespace LambdaCalculus.Named
 open Term
 
 /-- A variable in a term is either free or bound. -/
-lemma Term.vars_either_fv_or_bv [DecidableEq Var] {m : Term Var} :
+theorem vars_either_fv_or_bv [DecidableEq Var] {m : Term Var} :
     m.vars = m.fv ∪ m.bv := by
   induction m <;> grind [fv, bv, vars]
 
 /-- Renaming an unused variable has no effect. -/
 @[simp]
-lemma Term.rename_unused [DecidableEq Var] {m : Term Var} {x y : Var} :
+theorem rename_unused [DecidableEq Var] {m : Term Var} {x y : Var} :
   x ∉ m.vars → m.rename x y = m := by
   induction m <;> grind [vars, rename]
 
 /-- Renaming a variable to itself has no effect. -/
 @[simp]
-lemma Term.rename_same [DecidableEq Var] {m : Term Var} {x : Var} :
+theorem rename_same [DecidableEq Var] {m : Term Var} {x : Var} :
   m.rename x x = m := by
   induction m <;> grind [vars, rename]
 
 /-- Renaming a used variable changes the set of variables. -/
 @[simp]
-lemma Term.rename_vars_used [DecidableEq Var] {m : Term Var} {x y : Var} :
+theorem rename_vars_used [DecidableEq Var] {m : Term Var} {x y : Var} :
   x ∈ m.vars → (m.rename x y).vars = m.vars.erase x ∪ {y} := by
   induction m with
   | var z => grind [vars, rename]
@@ -49,39 +49,46 @@ lemma Term.rename_vars_used [DecidableEq Var] {m : Term Var} {x y : Var} :
   | app m n ihm ihn =>
     intro hx
     by_cases hxm : x ∈ m.vars
-    · by_cases hxn : x ∈ n.vars
-      · grind [vars, rename]
-      · grind [vars, rename, rename_unused]
-    · have hxn : x ∈ n.vars := by
-        grind [vars]
+    · by_cases hxn : x ∈ n.vars <;> grind [vars, rename, rename_unused]
+    · have hxn : x ∈ n.vars := by grind [vars]
       grind [vars, rename, rename_unused]
 
 /-- Renaming removes the variable. -/
-lemma Term.rename_remove [DecidableEq Var] {m : Term Var} {x y : Var} :
+theorem rename_remove [DecidableEq Var] {m : Term Var} {x y : Var} :
   x ≠ y → x ∉ (m.rename x y).vars := by
   intro hxy
   by_cases hx : x ∈ m.vars <;> grind [rename_vars_used, rename_unused]
 
-/-- Renaming changes set of variables. -/
-lemma Term.rename_vars [DecidableEq Var] {m : Term Var} {x y : Var} :
-  (m.rename x y).vars ⊆ m.vars \ {x} ∪ {y} := by
+/-- The set of variables after renaming. -/
+theorem rename_vars [DecidableEq Var] {m : Term Var} {x y : Var} :
+  (m.rename x y).vars = m.vars \ {x} ∪ (if x ∈ m.vars then {y} else ∅) := by
   by_cases x ∈ m.vars <;> grind [vars, rename, rename_unused, rename_vars_used]
+
+/-- The set of free variables after renaming. -/
+theorem rename_fv [DecidableEq Var] {m : Term Var} {x y : Var} :
+  y ∉ m.vars → (m.rename x y).fv = m.fv \ {x} ∪ (if x ∈ m.fv then {y} else ∅) := by
+  induction m <;> grind [fv, vars, rename, vars_either_fv_or_bv]
 
 /-- Concatenation of renaming. -/
 @[simp]
-lemma Term.rename_concat [DecidableEq Var] {m : Term Var} {x y z : Var} :
+theorem rename_concat [DecidableEq Var] {m : Term Var} {x y z : Var} :
   y ∉ m.vars → (m.rename x y).rename y z = m.rename x z := by
   induction m <;> grind [vars, rename]
 
 /-- Commutativity of renaming. -/
-@[simp]
-lemma Term.rename_comm [DecidableEq Var] {m : Term Var} {x y z w : Var} :
+theorem rename_comm [DecidableEq Var] {m : Term Var} {x y z w : Var} :
   x ≠ z → y ∉ m.vars ∪ {x, z} → w ∉ m.vars ∪ {x, z} →
   (m.rename x y).rename z w = (m.rename z w).rename x y := by
   induction m <;> grind [vars, rename]
 
+@[grind ←]
+lemma induction_by_sizeOf {m n : Term Var} :
+  WellFoundedRelation.rel m n ↔
+  sizeOf m < sizeOf n := by
+  rfl
+
 /-- α-equivalent terms have the same size. -/
-lemma AlphaEquiv.eq_sizeOf [DecidableEq Var] {m n : Term Var} :
+theorem AlphaEquiv.eq_sizeOf [DecidableEq Var] {m n : Term Var} :
   m =α n → sizeOf m = sizeOf n := by
   intro h
   induction h with
@@ -89,10 +96,25 @@ lemma AlphaEquiv.eq_sizeOf [DecidableEq Var] {m n : Term Var} :
   | @abs y x1 x2 m1 m2 hy h ih =>
     simpa using ih
   | @app m1 n1 m2 n2 _ hm hn =>
-    grind [app.sizeOf_spec]
+    grind
+
+/-- α-equivalent terms have the same free variables. -/
+theorem AlphaEquiv.same_fv [DecidableEq Var] {m n : Term Var} :
+  m =α n → m.fv = n.fv := by
+  intro h
+  induction h with
+  | @var x => rfl
+  | @abs y x1 x2 m1 m2 hy h ih =>
+    rw [Term.fv, Term.fv]
+    have h1 : m1.fv \ {x1} = (m1.rename x1 y).fv \ {y} := by
+      grind [rename_fv, vars_either_fv_or_bv]
+    have h2 : (m2.rename x2 y).fv \ {y} = m2.fv \ {x2} := by
+      grind [rename_fv, vars_either_fv_or_bv]
+    grind
+  | @app m1 n1 m2 n2 h1 h2 ih1 ih2 => grind [Term.fv]
 
 /-- Reflexivity of α-equivalence. -/
-lemma AlphaEquiv.refl [DecidableEq Var] [HasFresh Var] (m : Term Var) : m =α m := by
+theorem AlphaEquiv.refl [DecidableEq Var] [HasFresh Var] (m : Term Var) : m =α m := by
   refine WellFounded.induction (C := fun m => m =α m) sizeOfWFRel.wf m ?_
   simp only; intro m ih
   cases m with
@@ -100,21 +122,14 @@ lemma AlphaEquiv.refl [DecidableEq Var] [HasFresh Var] (m : Term Var) : m =α m 
   | abs x m =>
     obtain ⟨z, hz⟩ := HasFresh.fresh_exists (m.vars ∪ {x})
     apply AlphaEquiv.abs (y := z)
-    <;> try grind [rename_unused, rename_vars, rename_concat]
-    · apply ih
-      change sizeOf (m.rename x z) < sizeOf (abs x m)
-      grind [rename.eq_sizeOf, abs.sizeOf_spec]
+    · grind [rename_vars]
+    apply ih
+    grind [rename.eq_sizeOf]
   | app m n =>
-    apply AlphaEquiv.app
-    · apply ih
-      change sizeOf m < sizeOf (app m n)
-      grind [rename.eq_sizeOf, app.sizeOf_spec]
-    · apply ih
-      change sizeOf n < sizeOf (app m n)
-      grind [rename.eq_sizeOf, app.sizeOf_spec]
+    apply AlphaEquiv.app <;> apply ih <;> grind
 
 /-- Symmetry of α-equivalence. -/
-lemma AlphaEquiv.symm [DecidableEq Var] [HasFresh Var] {m n : Term Var} :
+theorem AlphaEquiv.symm [DecidableEq Var] [HasFresh Var] {m n : Term Var} :
   m =α n → n =α m := by
   intro h
   induction h with
@@ -124,9 +139,8 @@ lemma AlphaEquiv.symm [DecidableEq Var] [HasFresh Var] {m n : Term Var} :
   | @app m1 n1 m2 n2 hwm1 hwn1 hwm2 hwn2 =>
     apply AlphaEquiv.app <;> assumption
 
-/-- Renaming under an abstraction body can be reordered against the outer renaming.
-    This lemma is used for the lemma below. -/
-lemma Term.rename_abs_body_comm [DecidableEq Var] {m : Term Var} {x y z w : Var} :
+/-- Commutativity of renaming, more general version. -/
+theorem rename_comm2 [DecidableEq Var] {m : Term Var} {x y z w : Var} :
   y ∉ m.vars ∪ {x, z} → w ∉ m.vars ∪ {x, y, z} →
   (m.rename x y).rename (if z = x then y else z) w = (m.rename z w).rename x y := by
   intro hy hw
@@ -135,44 +149,39 @@ lemma Term.rename_abs_body_comm [DecidableEq Var] {m : Term Var} {x y z w : Var}
   · grind [rename_comm]
 
 /-- Renaming α-equivalent terms produces α-equivalent terms. -/
-lemma AlphaEquiv.rename_preserve [DecidableEq Var] [HasFresh Var]
+theorem AlphaEquiv.rename_preserve [DecidableEq Var] [HasFresh Var]
   (m n : Term Var) (x y : Var) :
   y ∉ m.vars ∪ n.vars → m =α n → (m.rename x y) =α (n.rename x y) := by
   refine (WellFounded.induction sizeOfWFRel.wf m
     (C := fun m => ∀ (n : Term Var) (x y : Var), y ∉ m.vars ∪ n.vars →
       m =α n → (m.rename x y) =α (n.rename x y)) ?_) n x y
   intro m ih n x y hy h
-  by_cases hxy : y = x
+  by_cases hyx : y = x
   · grind [rename_same]
   cases h with
   | @var z => apply AlphaEquiv.refl
   | @abs z x1 x2 m1 m2 hz hbody =>
     obtain ⟨w, hw⟩ := HasFresh.fresh_exists (m1.vars ∪ m2.vars ∪ {x1, x2, x, y, z})
-    apply AlphaEquiv.abs (y := w) <;> try grind [rename_vars]
-    rw [rename_abs_body_comm, rename_abs_body_comm] <;> try grind [vars]
-    apply ih <;> try grind [vars, rename_vars]
-    · change sizeOf (m1.rename x1 w) < sizeOf (abs x1 m1)
-      grind [rename.eq_sizeOf, abs.sizeOf_spec]
-    · have hxzw : ((m1.rename x1 z).rename z w) =α ((m2.rename x2 z).rename z w) := by
-        apply ih <;> try grind [vars, rename_vars]
-        · change sizeOf (m1.rename x1 z) < sizeOf (abs x1 m1)
-          grind [rename.eq_sizeOf, abs.sizeOf_spec]
-      grind [rename_concat]
+    apply AlphaEquiv.abs (y := w)
+    · grind [rename_vars]
+    rw [rename_comm2, rename_comm2]
+    case neg.abs.a =>
+      apply ih
+      · grind [rename.eq_sizeOf]
+      · grind [vars, rename_vars]
+      · have hxzw : ((m1.rename x1 z).rename z w) =α ((m2.rename x2 z).rename z w) := by
+          apply ih <;> grind [vars, rename_vars, rename.eq_sizeOf]
+        grind [rename_concat]
+    all_goals grind [vars]
   | @app m1 n1 m2 n2 hm hn =>
-    apply AlphaEquiv.app
-    · apply ih m1 <;> try grind [vars]
-      · change sizeOf m1 < sizeOf (app m1 m2)
-        grind [app.sizeOf_spec]
-    · apply ih m2 <;> try grind [vars]
-      · change sizeOf m2 < sizeOf (app m1 m2)
-        grind [app.sizeOf_spec]
+    apply AlphaEquiv.app <;> apply ih <;> grind [vars]
 
 /-- Elimination rule for α-equivalence of abstractions.
     It states that if two abstractions are α-equivalent,
     then their bodies can be renamed to ``any'' fresh variable y and remain α-equivalent.
     This is sometimes easier to use than using by_cases on the equivalence,
     which can only produce the claim for ``some'' fresh y. -/
-lemma AlphaEquiv.abs_elim [DecidableEq Var] [HasFresh Var] {m1 m2 : Term Var} {x1 x2 y : Var} :
+theorem AlphaEquiv.abs_elim [DecidableEq Var] [HasFresh Var] {m1 m2 : Term Var} {x1 x2 y : Var} :
   y ∉ m1.vars ∪ m2.vars ∪ {x1, x2} → (abs x1 m1) =α (abs x2 m2) →
   (m1.rename x1 y) =α (m2.rename x2 y) := by
   intro hy h
@@ -185,7 +194,7 @@ lemma AlphaEquiv.abs_elim [DecidableEq Var] [HasFresh Var] {m1 m2 : Term Var} {x
       grind [rename_concat, rename_vars]
 
 /-- Transitivity of α-equivalence. -/
-lemma AlphaEquiv.trans [DecidableEq Var] [HasFresh Var] {m n p : Term Var} :
+theorem AlphaEquiv.trans [DecidableEq Var] [HasFresh Var] {m n p : Term Var} :
   m =α n → n =α p → m =α p := by
   refine (WellFounded.induction sizeOfWFRel.wf m
     (C := fun m => ∀ (n p : Term Var),
@@ -204,25 +213,20 @@ lemma AlphaEquiv.trans [DecidableEq Var] [HasFresh Var] {m n p : Term Var} :
       cases hnp' with
       | @abs z x2 x3 m2 m3 hz h2 =>
         apply AlphaEquiv.abs (y := w)
-        <;> try grind [vars, rename_unused, rename_vars, rename_concat]
-        · apply ih _ ?_ (m2.rename x2 w) <;> try grind [AlphaEquiv.abs_elim, vars, rename_vars]
-          change sizeOf (m1.rename x1 w) < sizeOf (abs x1 m1)
-          grind [rename.eq_sizeOf, abs.sizeOf_spec]
+        · grind [vars, rename_unused, rename_vars, rename_concat]
+        apply ih _ ?_ (m2.rename x2 w) <;>
+        grind [AlphaEquiv.abs_elim, vars, rename_vars, rename.eq_sizeOf]
   | app m1 m2 =>
     cases hmn with
     | @app m1 n1 m2 n2 hmn1 hmn2 =>
       cases hnp with
       | @app n1 p1 n2 p2 hnp1 hnp2 =>
         apply AlphaEquiv.app
-        · apply ih _ ?_ n1 <;> try grind [vars, rename_vars]
-          change sizeOf m1 < sizeOf (app m1 m2)
-          grind [app.sizeOf_spec]
-        · apply ih _ ?_ n2 <;> try grind [vars, rename_vars]
-          change sizeOf m2 < sizeOf (app m1 m2)
-          grind [app.sizeOf_spec]
+        · apply ih _ ?_ n1 <;> grind [vars, rename_vars]
+        · apply ih _ ?_ n2 <;> grind [vars, rename_vars]
 
-/-- Renaming a non-free variable result in an α-equivalent term. -/
-lemma AlphaEquiv.rename_non_fv [DecidableEq Var] [HasFresh Var] (m : Term Var) (x y : Var)
+/-- Renaming a non-free variable result in an α-equivalent term -/
+theorem AlphaEquiv.rename_non_fv [DecidableEq Var] [HasFresh Var] (m : Term Var) (x y : Var)
   (hxm : x ∉ m.fv) (hym : y ∉ m.vars) : m =α (m.rename x y) := by
   induction m with
   | var z =>
@@ -234,22 +238,34 @@ lemma AlphaEquiv.rename_non_fv [DecidableEq Var] [HasFresh Var] (m : Term Var) (
     · subst z
       simp only [rename, ↓reduceIte]
       obtain ⟨w, hw⟩ := HasFresh.fresh_exists (m.vars ∪ {x, y})
-      apply AlphaEquiv.abs (y := w)<;> try grind [rename_unused, rename_vars]
-      rw [rename_concat] <;> try grind [vars]
-      apply AlphaEquiv.refl
+      apply AlphaEquiv.abs (y := w)
+      · grind [rename_unused, rename_vars]
+      rw [rename_concat] <;> grind [vars, AlphaEquiv.refl]
     · simp only [rename, hzx, ↓reduceIte]
       obtain ⟨w, hw⟩ := HasFresh.fresh_exists (m.vars ∪ {x, y, z})
-      apply AlphaEquiv.abs (y := w) <;> try grind [rename_unused, rename_vars]
+      apply AlphaEquiv.abs (y := w)
+      · grind [rename_unused, rename_vars]
       apply AlphaEquiv.rename_preserve <;> grind [vars, rename_vars, fv]
   | app m1 m2 ih1 ih2 =>
     apply AlphaEquiv.app
     · apply ih1 <;> grind [vars, fv]
     · apply ih2 <;> grind [vars, fv]
 
+/-- Abstracting over an arbitrary non-free variable results in the same term, modulo α-equivalence. -/
+theorem AlphaEquiv.abs_non_fv [DecidableEq Var] [HasFresh Var] {m1 m2 : Term Var} {x1 x2 : Var} :
+  m1 =α m2 → x1 ∉ m1.fv → x2 ∉ m2.fv → (abs x1 m1) =α (abs x2 m2) := by
+  intro hm hx1 hx2
+  obtain ⟨y, hy⟩ := HasFresh.fresh_exists (m1.vars ∪ m2.vars ∪ {x1, x2})
+  apply AlphaEquiv.abs (y := y)
+  · grind
+  apply AlphaEquiv.trans (n := m1)
+  · grind [rename_non_fv, AlphaEquiv.symm]
+  apply AlphaEquiv.trans (n := m2) <;> grind [rename_non_fv]
+
 /-- Any `Term` can be obtained by filling a `Context` with a variable. This proves that `Context`
 completely captures the syntax of terms. -/
 theorem Context.complete (m : Term Var) :
-    ∃ (c : Context Var) (x : Var), m = (c.fill (Term.var x)) := by
+    ∃ (c : Context Var) (x : Var), m = (c.fill (var x)) := by
   induction m with
   | var x => exists hole, x
   | abs x n ih =>
@@ -261,6 +277,323 @@ theorem Context.complete (m : Term Var) :
     exists Context.appL c₁ n₂, x₁
     rw [ih₁, fill]
 
+/-- The set of variables after filling a context. -/
+theorem Context.fill_vars [DecidableEq Var] {c : Context Var} {m : Term Var} :
+  (c.fill m).vars = c.vars ∪ m.vars := by
+  induction c <;> grind [Context.fill, Context.vars, Term.vars]
+
+/-- α-equivalence is preserved under context filling. -/
+theorem AlphaEquiv.context [DecidableEq Var] [HasFresh Var] {m n : Term Var} {c : Context Var} :
+  m =α n → (c.fill m) =α (c.fill n) := by
+  intro h
+  induction c with
+  | hole => assumption
+  | abs x c ih =>
+    simp only [Context.fill]
+    obtain ⟨y, hy⟩ := HasFresh.fresh_exists (m.vars ∪ n.vars ∪ c.vars ∪ {x})
+    apply AlphaEquiv.abs (y := y) <;> grind [Context.fill_vars, rename_preserve]
+  | appL c m ih =>
+    apply AlphaEquiv.app <;> grind [AlphaEquiv.app, AlphaEquiv.refl, vars]
+  | appR m c ih =>
+    apply AlphaEquiv.app <;> grind [AlphaEquiv.app, AlphaEquiv.refl, vars]
+
+/-- The functional definition of substitution satisfies the relational definition of substitution. -/
+theorem Subst.function_to_relation [DecidableEq Var] [HasFresh Var] {m r : Term Var} {x : Var} :
+  m.Subst x r (m[x := r]) := by
+  refine WellFounded.induction (C := fun m => m.Subst x r (m[x := r])) sizeOfWFRel.wf m ?_
+  simp only; intro m ih
+  cases m with
+  | var y =>
+    by_cases hyx : y = x
+    · subst y
+      simp only [← subst_def, subst.eq_1, ↓reduceIte]
+      apply Subst.varHit
+    · simp [hyx]
+      grind [Subst.varMiss]
+  | abs y m =>
+    by_cases hyx : y = x
+    · subst y
+      simp only [← subst_def, subst.eq_2, ↓reduceIte]
+      apply Subst.absShadow
+    · simp only [← subst_def, subst.eq_2, hyx, ↓reduceIte, Finset.union_insert]
+      by_cases hyr : y ∈ r.fv
+      · simp only [hyr]
+        have hz := fresh_notMem (insert x (insert y (m.vars ∪ r.vars)))
+        set z := fresh (insert x (insert y (m.vars ∪ r.vars)))
+        apply Subst.alpha (m := abs z (m.rename y z)) (r := r) (n := abs z ((m.rename y z)[x := r]))
+        · have h1 : abs z (m.rename y z) = (abs y m).rename y z := by
+            simp [rename]
+          grind [AlphaEquiv.symm, AlphaEquiv.rename_non_fv, vars, fv]
+        · grind [AlphaEquiv.refl]
+        · grind [AlphaEquiv.refl]
+        · apply Subst.absIn
+          · grind [vars, fv, vars_either_fv_or_bv]
+          apply ih
+          grind [rename.eq_sizeOf]
+      · simp only [hyr]
+        apply Subst.absIn
+        · grind [vars, fv, vars_either_fv_or_bv]
+        apply ih
+        grind
+  | app m1 m2 =>
+    simp only [← subst_def, subst.eq_3]
+    apply Subst.app <;> apply ih <;> grind
+
+/-- substituting a non-free variable has no effect. -/
+theorem subst.non_free [DecidableEq Var] [HasFresh Var] {m r : Term Var} {x : Var} :
+  x ∉ m.fv → (m[x := r]) =α m := by
+  refine WellFounded.induction (C := fun m => x ∉ m.fv → (m[x := r]) =α m) sizeOfWFRel.wf m ?_
+  simp only; intro m ih hx
+  cases m with
+  | var y =>
+    have hyx : y ≠ x := by
+      grind [fv]
+    simp only [← subst_def, subst.eq_1, hyx, ↓reduceIte]
+    apply AlphaEquiv.var
+  | abs y m =>
+    by_cases hyx : y = x
+    · subst y
+      simp only [← subst_def, subst.eq_2, ↓reduceIte]
+      apply AlphaEquiv.refl
+    · by_cases hyr : y ∈ r.fv
+      · simp only [← subst_def, subst.eq_2, hyx, ↓reduceIte, hyr, not_true_eq_false,
+          Finset.union_insert, Finset.union_singleton]
+        have hz := fresh_notMem (insert x (insert y (m.vars ∪ r.vars)))
+        set z := fresh (insert x (insert y (m.vars ∪ r.vars)))
+        obtain ⟨w, hw⟩ := HasFresh.fresh_exists (m.vars ∪ r.vars ∪ ((m.rename y z).subst x r).vars
+          ∪ {x, y, z})
+        apply AlphaEquiv.abs (y := w)
+        · grind [vars, rename_unused, rename_vars]
+        apply AlphaEquiv.trans (n := ((m.rename y z).rename z w))
+        · apply AlphaEquiv.rename_preserve
+          · grind [vars, rename_vars, fv]
+          apply ih <;> grind [fv, rename_fv, rename.eq_sizeOf]
+        · grind [rename_concat, AlphaEquiv.refl]
+      · simp only [← subst_def, subst.eq_2, hyx, ↓reduceIte, hyr, not_false_eq_true]
+        apply AlphaEquiv.context (c := Context.abs y Context.hole)
+        apply ih <;> grind [fv]
+  | app m1 m2 =>
+    simp only [← subst_def, subst.eq_3]
+    apply AlphaEquiv.app <;> apply ih <;> grind [fv]
+
+/-- Renaming an abstraction leads to an α-equivalent term. -/
+theorem AlphaEquiv.abs_rename [DecidableEq Var] [HasFresh Var] {m : Term Var} {x y : Var} :
+  y ∉ m.vars ∪ {x} → (abs x m) =α (abs y (m.rename x y)) := by
+  intro hy
+  obtain ⟨z, hz⟩ := HasFresh.fresh_exists (m.vars ∪ {x, y})
+  apply AlphaEquiv.abs (y := z) <;> grind [vars, rename_vars, rename_concat, AlphaEquiv.refl]
+
+lemma AlphaEquiv.subst_abs_fresh_helper [DecidableEq Var] [HasFresh Var]
+  {m r : Term Var} {x y z : Var} :
+  z ∉ m.vars ∪ r.vars ∪ {x, y} →
+  ((abs y m)[x := r]) =α (abs z ((m.rename y z)[x := r]))
+  ∧ (y ∉ r.fv ∪ {x} → (abs y (m[x := r])) =α (abs z ((m.rename y z)[x := r]))) := by
+  refine (WellFounded.induction sizeOfWFRel.wf m
+    (C := fun m => ∀ (r : Term Var) (x y z : Var),
+      z ∉ m.vars ∪ r.vars ∪ {x, y} →
+  ((abs y m)[x := r]) =α (abs z ((m.rename y z)[x := r]))
+  ∧ (y ∉ r.fv ∪ {x} → (abs y (m[x := r])) =α (abs z ((m.rename y z)[x := r])))) ?_) r x y z
+  intro m ih r x y z hz
+  have hright : ∀ (m' : Term Var) (y' : Var), sizeOf m' = sizeOf m → z ∉ m'.vars ∪ r.vars ∪ {x, y'}
+    → y' ∉ r.fv ∪ {x} → (Term.abs y' (m'[x:=r])) =α (Term.abs z ((m'.rename y' z)[x:=r])) := by
+    intro m' y' hm' hz hy'
+    cases m' with
+    | var w =>
+      by_cases hwx : w = x
+      · subst w
+        have hxy' : x ≠ y' := by grind
+        rw [rename]
+        simp only [← subst_def, subst.eq_1, ↓reduceIte, hxy']
+        apply abs_non_fv <;> grind [vars_either_fv_or_bv, AlphaEquiv.refl]
+      · simp only [← subst_def, subst.eq_1, hwx, ↓reduceIte]
+        rw [rename]
+        by_cases hwy' : w = y'
+        · subst w
+          have hzx : z ≠ x := by grind
+          simp only [↓reduceIte, subst.eq_1, hzx]
+          obtain ⟨v, hv⟩ := HasFresh.fresh_exists ({y', z})
+          apply AlphaEquiv.abs (y := v) <;> grind [vars, rename, AlphaEquiv.var]
+        · simp only [hwy', ↓reduceIte, subst.eq_1, hwx]
+          apply abs_non_fv <;> grind [vars_either_fv_or_bv, AlphaEquiv.refl, Term.fv]
+    | app m1 m2 =>
+      obtain ⟨w, hw⟩ := HasFresh.fresh_exists
+        ((m1.app m2)[x := r].vars ∪ (((m1.app m2).rename y' z)[x := r]).vars
+        ∪ m1[x := r].vars ∪ m2[x := r].vars ∪ (m1.rename y' z)[x := r].vars
+        ∪ (m2.rename y' z)[x := r].vars ∪ {y', z})
+      apply AlphaEquiv.abs (y := w)
+      · grind
+      simp only [← subst_def, subst.eq_3, rename]
+      apply AlphaEquiv.app <;> apply AlphaEquiv.abs_elim <;> grind [vars, rename_vars]
+    | abs w m1 =>
+      by_cases hwy' : w = y'
+      · subst w
+        rw [rename]
+        have hy'x : y' ≠ x := by grind
+        have hy'r : y' ∉ r.fv := by grind
+        have hzx : z ≠ x := by grind
+        have hzr : z ∉ r.fv := by grind [vars_either_fv_or_bv]
+        simp only [← subst_def, subst.eq_2, hy'x, ↓reduceIte, hy'r, not_false_eq_true, hzx, hzr]
+        apply abs_non_fv
+        · apply (ih _ _ _ _ _ _ _).right <;> grind [vars]
+        · grind [fv]
+        · grind [fv]
+      · rw [rename]
+        simp only [hwy', ↓reduceIte]
+        by_cases hwx : w = x
+        · subst w
+          simp only [← subst_def, subst, ↓reduceIte]
+          apply AlphaEquiv.trans (n := Term.abs z ((Term.abs x m1).rename y' z))
+          · grind [AlphaEquiv.abs_rename]
+          · grind [rename, AlphaEquiv.refl]
+        · by_cases hwr : w ∈ r.fv
+          · obtain ⟨v, hv⟩ := HasFresh.fresh_exists (m1.vars ∪ r.vars ∪ {x, y', z, w})
+            have hl : (Term.abs y' (((Term.abs w m1)[x := r]))) =α
+                (Term.abs y' (Term.abs v ((m1.rename w v)[x := r]))) := by
+              apply AlphaEquiv.context (c := Context.abs y' Context.hole)
+              apply (ih _ _ _ _ _ _ _).left <;> grind
+            have hr : (Term.abs z (Term.abs v (((m1.rename y' z).rename w v)[x := r])))
+              =α (Term.abs z ((Term.abs w (m1.rename y' z))[x := r])) := by
+              apply AlphaEquiv.context (c := Context.abs z Context.hole)
+              apply AlphaEquiv.symm
+              apply (ih _ _ _ _ _ _ _).left <;> grind [rename_vars, rename.eq_sizeOf]
+            have hmid : (abs y' (abs v ((m1.rename w v)[x := r]))) =α
+                (abs z (abs v (((m1.rename y' z).rename w v)[x := r]))) := by
+              obtain ⟨u, hu⟩ := HasFresh.fresh_exists
+                ((Term.abs v ((m1.rename w v)[x := r])).vars ∪
+                (Term.abs v (((m1.rename y' z).rename w v)[x := r])).vars ∪
+                ((m1.rename w v).rename y' z)[x:=r].vars ∪ {y', z})
+              apply AlphaEquiv.abs (y := u)
+              · grind
+              · have hvy' : v ≠ y' := by grind
+                have hvz : v ≠ z := by grind
+                simp only [rename, hvy', hvz, ↓reduceIte]
+                apply AlphaEquiv.context (c := Context.abs v Context.hole)
+                apply AlphaEquiv.trans (n := (((m1.rename w v).rename y' z)[x := r]).rename z u)
+                · apply AlphaEquiv.abs_elim
+                  · grind  [vars]
+                  · apply (ih _ _ _ _ _ _ _).right <;> grind [vars, rename_vars, rename.eq_sizeOf]
+                · apply rename_preserve
+                  · grind [vars]
+                  · rw [rename_comm] <;> grind [vars, AlphaEquiv.refl]
+            exact AlphaEquiv.trans hl <| AlphaEquiv.trans hmid hr
+          · obtain ⟨v, hv⟩ := HasFresh.fresh_exists
+              (m1[x:=r].vars ∪ (m1.rename y' z)[x:=r].vars ∪ ((Term.abs w m1)[x := r]).vars ∪
+              ((Term.abs w (m1.rename y' z))[x := r]).vars ∪ {y', z})
+            apply AlphaEquiv.abs (y := v)
+            · grind [vars, rename_vars]
+            · have hwz : w ≠ z := by grind [vars]
+              simp only [← subst_def, subst, hwx, ↓reduceIte, hwr, not_false_eq_true, rename, hwy',
+                hwz]
+              apply AlphaEquiv.context (c := Context.abs w Context.hole)
+              apply AlphaEquiv.abs_elim <;> grind [vars]
+  have hleft : ((Term.abs y m)[x:=r]) =α (Term.abs z ((m.rename y z)[x:=r])) := by
+    by_cases hyx : y = x
+    · subst y
+      simp only [← subst_def, subst.eq_2, ↓reduceIte]
+      obtain ⟨w, hw⟩ := HasFresh.fresh_exists (m.vars ∪ r.vars ∪ ((m.rename x z).subst x r).vars ∪
+        {x, z})
+      apply AlphaEquiv.abs (y := w)
+      · grind [vars, rename_unused, rename_vars]
+      · apply AlphaEquiv.trans (n := ((m.rename x z).rename z w))
+        · grind [AlphaEquiv.refl, rename_concat]
+        · apply AlphaEquiv.rename_preserve
+          · grind [rename_vars]
+          · apply AlphaEquiv.symm
+            apply subst.non_free
+            grind [fv, rename_fv, rename.eq_sizeOf]
+    · by_cases hyr : y ∈ r.fv
+      · simp only [← subst_def, subst.eq_2, hyx, ↓reduceIte, hyr, not_true_eq_false,
+          Finset.union_insert, Finset.union_singleton]
+        have hw := fresh_notMem (insert x (insert y (m.vars ∪ r.vars)))
+        set w := fresh (insert x (insert y (m.vars ∪ r.vars)))
+        by_cases hzw' : z = w
+        · subst z
+          apply AlphaEquiv.refl
+        · apply AlphaEquiv.trans (n := (abs z (((m.rename y w).rename w z)[x := r])))
+          · apply hright <;>
+              grind [rename.eq_sizeOf, vars_either_fv_or_bv, rename_vars]
+          · rw [rename_concat] <;> grind [AlphaEquiv.refl]
+      · simp only [← subst_def, subst.eq_2, hyx, ↓reduceIte, hyr, not_false_eq_true]
+        apply hright <;> grind
+  exact ⟨hleft, hright m y (by rfl) (by grind)⟩
+
+/-- Modulo α-equivalence, substituting an abstraction falls back to the fresh variable case only.
+    With this lemma, the three cases in the definition of subst can be reduced to one.
+-/
+theorem AlphaEquiv.subst_abs_fresh [DecidableEq Var] [HasFresh Var]
+  {m r : Term Var} {x y z : Var} :
+  z ∉ m.vars ∪ r.vars ∪ {x, y} →
+  ((abs y m)[x := r]) =α (abs z ((m.rename y z)[x := r])) := by
+  grind [AlphaEquiv.subst_abs_fresh_helper]
+
+/-- Substituting α-equivalent terms produces α-equivalent terms. -/
+theorem subst.preserve_AlphaEquiv [DecidableEq Var] [HasFresh Var]
+  {m m' r r' : Term Var} {x : Var} :
+  m =α m' → r =α r' → (m[x := r]) =α (m'[x := r']) := by
+  refine (WellFounded.induction sizeOfWFRel.wf m
+    (C := fun m => ∀ (m' r r' : Term Var) (x : Var),
+      m =α m' → r =α r' → (m[x := r]) =α (m'[x := r'])) ?_) m' r r' x
+  intro m ih m' r r' x hmm' hrr'
+  have hmm'' := hmm'
+  cases hmm'' with
+  | @var y =>
+    by_cases hyx : y = x
+    · simp only [← subst_def, subst, ↓reduceIte, hyx]
+      assumption
+    · simp only [← subst_def, subst, hyx]
+      apply AlphaEquiv.refl
+  | @abs z y y' m m' hz h1 =>
+    obtain ⟨w, hw⟩ := HasFresh.fresh_exists (m.vars ∪ m'.vars ∪ r.vars ∪ r'.vars ∪ {x, y, y'})
+    have h2 : ((abs y m)[x := r]) =α (abs w ((m.rename y w)[x := r])) := by
+      grind [AlphaEquiv.subst_abs_fresh]
+    have h2' : ((abs y' m')[x := r']) =α
+        (abs w ((m'.rename y' w)[x := r'])) := by
+      grind [AlphaEquiv.subst_abs_fresh]
+    have hbody : (m.rename y w) =α (m'.rename y' w) := by
+      apply AlphaEquiv.abs_elim <;> grind
+    have h3 : (abs w ((m.rename y w)[x := r])) =α (abs w ((m'.rename y' w)[x := r'])) := by
+      apply AlphaEquiv.context (c := Context.abs w Context.hole)
+      apply ih <;> grind [rename.eq_sizeOf]
+    apply AlphaEquiv.trans (n := (abs w ((m.rename y w)[x := r]))) <;> try assumption
+    apply AlphaEquiv.trans (n := (abs w ((m'.rename y' w)[x := r']))) <;> try assumption
+    apply AlphaEquiv.symm
+    assumption
+  | @app m m' n n' hm hn =>
+    simp only [← subst_def, subst]
+    apply AlphaEquiv.app <;> apply ih <;> grind
+
+/-- The relational definition of substitution coincides with the functional definition of
+    substitution, modulo α-equivalence. -/
+theorem Subst.relation_function_iff [DecidableEq Var] [HasFresh Var] {m n r : Term Var} {x : Var} :
+  m.Subst x r n ↔ n =α (m[x := r]) := by
+  constructor
+  · intro h
+    induction h with
+    | @varHit x r =>
+      simp only [← subst_def, subst, ↓reduceIte]
+      apply AlphaEquiv.refl
+    | @varMiss x y r hyx =>
+      simp only [← subst_def, subst, hyx, ↓reduceIte]
+      apply AlphaEquiv.refl
+    | @absShadow x m r =>
+      simp only [← subst_def, subst, ↓reduceIte]
+      apply AlphaEquiv.refl
+    | @absIn x y m r m' hy h ih =>
+      have hyx : y ≠ x := by grind
+      have hyr : y ∉ r.fv := by grind
+      simp only [← subst_def, subst, hyx, ↓reduceIte, hyr, not_false_eq_true]
+      apply AlphaEquiv.context (c := Context.abs y Context.hole)
+      assumption
+    | @app m n x r m' n' h1 h2 ih1 ih2 =>
+      simp only [← subst_def, subst]
+      apply AlphaEquiv.app <;> assumption
+    | @alpha m m' r r' n n' x hm hr hn h ih =>
+      apply AlphaEquiv.trans (n := n)
+      · grind [AlphaEquiv.symm]
+      apply AlphaEquiv.trans (n := m[x := r]) <;> grind [subst.preserve_AlphaEquiv]
+  · intro h
+    apply Subst.alpha (m := m) (r := r) (n := m[x := r]) <;> grind [AlphaEquiv.symm,
+      AlphaEquiv.refl, Subst.function_to_relation]
 
 end LambdaCalculus.Named
 
